theories/Pre_orders/May/LiftMay.v
@@ -1,0 +1,227 @@
+(*
+   Copyright (c) 2024 Nomadic Labs
+   Copyright (c) 2024 Paul Laforgue <paul.laforgue@nomadic-labs.com>
+   Copyright (c) 2024 Léo Stefanesco <leo.stefanesco@mpi-sws.org>
+   Copyright (c) 2025 Gaëtan Lopez <glopez@irif.fr>
+
+   Permission is hereby granted, free of charge, to any person obtaining a copy
+   of this software and associated documentation files (the "Software"), to deal
+   in the Software without restriction, including without limitation the rights
+   to use, copy, modify, merge, publish, distribute, sublicense, and/or sell
+   copies of the Software, and to permit persons to whom the Software is
+   furnished to do so, subject to the following conditions:
+
+   The above copyright notice and this permission notice shall be included in all
+   copies or substantial portions of the Software.
+
+   THE SOFTWARE IS PROVIDED "AS IS", WITHOUT WARRANTY OF ANY KIND, EXPRESS OR
+   IMPLIED, INCLUDING BUT NOT LIMITED TO THE WARRANTIES OF MERCHANTABILITY,
+   FITNESS FOR A PARTICULAR PURPOSE AND NONINFRINGEMENT. IN NO EVENT SHALL THE
+   AUTHORS OR COPYRIGHT HOLDERS BE LIABLE FOR ANY CLAIM, DAMAGES OR OTHER
+   LIABILITY, WHETHER IN AN ACTION OF CONTRACT, TORT OR OTHERWISE, ARISING FROM,
+   OUT OF OR IN CONNECTION WITH THE SOFTWARE OR THE USE OR OTHER DEALINGS IN THE
+   SOFTWARE.
+*)
+
+From Coq.Program Require Import Equality.
+From stdpp Require Import base countable finite gmap list 
+                        finite base decidable finite gmap gmultiset.
+From Must Require Import ForAllHelper gLts Bisimulation Lts_OBA Lts_OBA_FB Lts_FW Testing_Predicate 
+  May CodePurification Termination 
+  InteractionBetweenLts MultisetLTSConstruction ParallelLTSConstruction ForwarderConstruction FiniteImageLTS.
+From Must Require Import ActTau.
+
+Lemma may_non_blocking_action_swap_l_fw_eq `{
+  @gLtsObaFW P A H gLtsP gLtsEqP gLtsObaP, 
+  @gLtsObaFB E A H gLtsE gLtsEqE gLtsObaE, !Testing_Predicate E A attaboy}
+
+  `{@Prop_of_Inter P E A parallel_inter H gLtsP gLtsE}
+
+  (p1 p2 : P) (e1 e2 : E) (η : A) :
+  non_blocking η -> p1 ⟶⋍[η] p2 -> e1 ⟶⋍[η] e2 -> may p1 e2
+    -> may p2 e1.
+Proof.
+Admitted.
+
+Lemma may_non_blocking_action_swap_r_fw_eq`{
+  @gLtsObaFW P A H gLtsP gLtsEqP gLtsObaP, 
+  @gLtsObaFB E A H gLtsE gLtsEqE gLtsObaE, !Testing_Predicate E A attaboy}
+
+  `{@Prop_of_Inter P E A parallel_inter H gLtsP gLtsE}
+
+  (p1 p2 : P) (e1 e2 : E) (η : A) :
+  non_blocking η -> p1 ⟶⋍[η] p2 -> e1 ⟶⋍[η] e2 -> may p2 e1
+    -> may p1 e2.
+Proof.
+Admitted.
+
+Lemma may_non_blocking_action_swap_l_fw `{
+  @gLtsObaFW P A H gLtsP gLtsEqP gLtsObaP, 
+  @gLtsObaFB E A H gLtsE gLtsEqE gLtsObaE, !Testing_Predicate E A attaboy}
+
+  `{@Prop_of_Inter P E A parallel_inter H gLtsP gLtsE}
+
+  (p1 p2 : P) (e1 e2 : E) (η : A) :
+  non_blocking η -> p1 ⟶[η] p2 -> e1 ⟶[η] e2 -> may p1 e2 
+    -> may p2 e1.
+Proof.
+  intros. eapply may_non_blocking_action_swap_l_fw_eq; eauto; eexists; split; eauto; reflexivity.
+Qed.
+
+Lemma may_non_blocking_action_swap_r_fw `{
+  @gLtsObaFW P A H gLtsP gLtsEqP gLtsObaP, 
+  @gLtsObaFB E A H gLtsE gLtsEqE gLtsObaE, !Testing_Predicate E A attaboy}
+
+  `{@Prop_of_Inter P E A parallel_inter H gLtsP gLtsE}
+
+  (p1 p2 : P) (e1 e2 : E) (η : A) :
+  non_blocking η -> p1 ⟶[η] p2 -> e1 ⟶[η] e2 -> may p2 e1
+    -> may p1 e2.
+Proof.
+  intros.
+  eapply may_non_blocking_action_swap_r_fw_eq; eauto; eexists; split; eauto; reflexivity.
+Qed.
+
+Lemma nf_may_fw_l `{
+  @gLtsObaFB P A H gLtsP M K, !FiniteImagegLts P A,
+  @gLtsObaFB E A H gLtsE Y V, !Testing_Predicate E A attaboy}
+
+  `{@Prop_of_Inter P (mb A) A fw_inter H gLtsP MbgLts}
+  `{@Prop_of_Inter (P * mb A) E A parallel_inter H (inter_lts fw_inter) gLtsE}
+
+  m1 m2 (p : P) (e e' : E) : e ⟿{m1} e' -> may (p, m1 ⊎ m2) e' -> may (p, m2) e.
+Proof.
+  revert p e e' m2.
+  induction m1 using gmultiset_ind; intros p e e' m2 hmo hm.
+  - inversion hmo; subst.
+    rewrite gmultiset_disj_union_left_id in hm.
+    symmetry in eq. eapply must_eq_client; eauto.
+    multiset_solver.
+  - assert (non_blocking x) as nb. eapply nb_with_strip; eauto. multiset_solver.
+    assert (x ∈ {[+ x +]} ⊎ m1) as mem by multiset_solver.
+    eapply aux0 in mem as (e0 & l0); eauto.
+    eapply (aux3_) in hmo as (t & hwo & heq); eauto.
+    eapply (may_non_blocking_action_swap_l_fw_eq ).
+    exact nb. exists (p ▷ m2). split. 
+    apply (ParRight (ActExt x) p ({[+ x +]} ⊎ m2) (m2)).
+    unfold lts_step;simpl.
+    eapply lts_multiset_minus; eauto. 
+    reflexivity. exists e0. split. eassumption. reflexivity.
+    eapply IHm1. eassumption. eapply must_eq_client. symmetry. eassumption.
+    now replace (m1 ⊎ ({[+ x +]} ⊎ m2)) with ({[+ x +]} ⊎ m1 ⊎ m2) by multiset_solver.
+Qed.
+
+Lemma nf_may_fw_r `{
+  @gLtsObaFB P A H gLtsP gLtsEqP gLtsObaP, !FiniteImagegLts P A ,
+  @gLtsObaFB E A H gLtsE gLtsEqE gLtsObaE, !Testing_Predicate E A attaboy}
+
+  `{@Prop_of_Inter P (mb A) A fw_inter H gLtsP MbgLts}
+  `{@Prop_of_Inter (P * mb A) E A parallel_inter H (inter_lts fw_inter) gLtsE}
+
+  (p : P) (e e' : E) m1 m2 : 
+  e ⟿{m1} e' -> may (p, m2) e -> may (p, m1 ⊎ m2) e'.
+Proof.
+  intro hwo. revert p m2.
+  dependent induction hwo; intros q m2 hm.
+  rename p into e, q into p.
+  - rewrite gmultiset_disj_union_left_id. eapply must_eq_client; eauto.
+  - assert (may (q, {[+ η +]} ⊎ m2) p2).
+    { admit. }
+    replace ({[+ η +]} ⊎ m ⊎ m2) with (m ⊎ ({[+ η +]} ⊎ m2)) by multiset_solver.
+    eapply IHhwo. eassumption.
+Admitted.
+
+Lemma nf_may_fw `{
+  @gLtsObaFB P A H gLtsP M K, !FiniteImagegLts P A ,
+  @gLtsObaFB E A H gLtsE Y V , !Testing_Predicate E A attaboy}
+
+  `{@Prop_of_Inter P (mb A) A fw_inter H gLtsP MbgLts}
+  `{@Prop_of_Inter (P * mb A) E A parallel_inter H (inter_lts fw_inter) gLtsE}
+
+  (p : P) (e e' : E) m : 
+  e ⟿{m} e' -> may (p, m) e' <-> may (p, ∅) e.
+Proof.
+  intros. split; intro hm.
+  - eapply nf_may_fw_l; eauto. now rewrite gmultiset_disj_union_right_id.
+  - rewrite <- gmultiset_disj_union_right_id. eapply nf_may_fw_r; eassumption.
+Qed.
+
+Lemma may_to_may_fw `{
+  @gLtsObaFB P A H gLtsP gLtsEqP gLtsObaP, !FiniteImagegLts P A,
+  @gLtsObaFB E A H gLtsE gLtsEqE gLtsObaE, !Testing_Predicate E A attaboy}
+
+  `{@Prop_of_Inter P (mb A) A fw_inter H gLtsP MbgLts}
+  `{@Prop_of_Inter (P * mb A) E A parallel_inter H (inter_lts fw_inter) gLtsE}
+  `{@Prop_of_Inter P E A parallel_inter H gLtsP gLtsE}
+
+  (p : P) (e : E) (m : mb A) :
+  may p e -> m = lts_oba_mo e -> forall e', e ⟿{m} e' 
+    -> may (p, m) e'.
+Proof.
+  intros hm. revert m.
+  dependent induction hm.
+  - admit.
+  - admit.
+  - admit.
+  - admit.
+Admitted.
+
+Lemma may_fw_to_may `{
+  @gLtsObaFB P A H gLtsP gLtsEqP gLtsObaP, !FiniteImagegLts P A,
+  @gLtsObaFB E A H gLtsE gLtsEqE gLtsObaE, !Testing_Predicate E A attaboy}
+
+  `{@Prop_of_Inter P (mb A) A fw_inter H gLtsP MbgLts}
+  `{@Prop_of_Inter (P * mb A) E A parallel_inter H (inter_lts fw_inter) gLtsE}
+  `{@Prop_of_Inter P E A parallel_inter H gLtsP gLtsE}
+
+  (p : P) (e : E) : may (p, ∅) e -> may p e.
+Proof.
+  intro hm. dependent induction hm.
+  - admit.
+  - admit.
+  - admit.
+  - admit.
+Admitted.
+
+Lemma may_iff_may_fw `{
+  @gLtsObaFB P A H gLtsP gLtsEqP gLtsObaP, !FiniteImagegLts P A,
+  @gLtsObaFB E A H gLtsE gLtsEqE gLtsObaE , !Testing_Predicate E A attaboy}
+
+  `{@Prop_of_Inter P (mb A) A fw_inter H gLtsP MbgLts}
+  `{@Prop_of_Inter (P * mb A) E A parallel_inter H (inter_lts fw_inter) gLtsE}
+  `{@Prop_of_Inter P E A parallel_inter H gLtsP gLtsE}
+
+  (p : P) (e : E) :
+  may p e <-> may (p, ∅) e.
+Proof.
+  split; intro hm.
+  - edestruct (lts_oba_mo_strip e) as (e' & hmo).
+    eapply nf_may_fw_l. eassumption.
+    rewrite gmultiset_disj_union_right_id.
+    eapply may_to_may_fw. eassumption. reflexivity. eassumption.
+  - eapply may_fw_to_may; eauto.
+Qed.
+
+Lemma lift_fw_ctx_pre `{
+    @gLtsObaFB P A H gLtsP gLtsEqP gLtsObaP, !FiniteImagegLts P A,
+    @gLtsObaFB Q A H gLtsQ gLtsEqQ gLtsObaQ, !FiniteImagegLts Q A,
+    @gLtsObaFB E A H gLtsE gLtsEqE gLtsObaE, !Testing_Predicate E A attaboy}
+
+  `{@Prop_of_Inter P (mb A) A fw_inter H gLtsP MbgLts}
+
+  `{@Prop_of_Inter (P * mb A) E A parallel_inter H (inter_lts fw_inter) gLtsE}
+
+  `{@Prop_of_Inter P E A parallel_inter H gLtsP gLtsE}
+
+  `{@Prop_of_Inter Q (mb A) A fw_inter H gLtsQ MbgLts}
+
+  `{@Prop_of_Inter (Q * mb A) E A parallel_inter H (inter_lts fw_inter) gLtsE}
+
+  `{@Prop_of_Inter Q E A parallel_inter H gLtsQ gLtsE}
+
+  (p : P) (q : Q) : p ⊑ q <-> (p, ∅) ⊑ (q, ∅).
+Proof.
+  split; intros hctx e hm%may_iff_may_fw. 
+  - rewrite <- may_iff_may_fw. eauto.
+  - rewrite may_iff_may_fw. eauto.
+Qed.
